test if an induction principle on denote is useful
Export some lemmas

add provide notation

Remove exports inside the framework.
Introduce notations for Provide and MayProvide and rework proofs around those.
Remove Generalizable All Variables (antipattern).

theories/Effect.v
@@ -4,7 +4,11 @@
 
 (* Copyright (C) 2018–2020 ANSSI *)
 
-From FreerDPS Require Import Init.
+From mathcomp Require Import ssreflect ssrfun.
+From monae Require Import hierarchy.
+From Stdlib Require Import Program.
+
+Local Open Scope monae_scope.
 
 (** * Definition  *)
 
@@ -56,54 +60,51 @@ Arguments Put [s] (x).
     and [E]. *)
 
 (** * Polymorphic Effect Composites *)
-
-(** When defining general-purpose impure computations that we expect to reuse in
-    different context, we want to leave the effect as a parameter, and rather
-    express the constraints in terms of effect availability.  We tackle this
-    challenge by means of _effect composites_.
-
-    - We say an effect composite [Fx] _provides_ a concrete effect [F]
-      when there exists a function [inj_p : forall α, F α -> Fx α].
-    - Conversely, we can determine if a primitive of an effect composite [Fx]
-      is forwarded to a concrete effect [F] when there exists a function
-      [proj_p : forall α, Fx α -> option (F a)].
-
-    We encode this mechanics using two type classes: [MayProvide], and
-    [Provide]. *)
-
 Class MayProvide (Fx F : effect) : Type :=
-  { proj_p {α} (e : Fx α) : option (F α)
+  { proj: Fx ~~> option \o F (* retraction *)
   }.
+Arguments proj {_ _ _ _} _.
 
-Class Provide (Fx F : effect) `{MayProvide Fx F} : Type :=
-  { inj_p {α} (e : F α) : Fx α
-  ; proj_inj_p_equ {α} (e : F α) : proj_p (inj_p e) = Some e
-  }.
+Notation "F -<? Fx" := (MayProvide Fx F)
+  (at level 92, left associativity) : type_scope.
+
+Class Provide (Fx F : effect) : Type :=
+  { may_prov :: F -<? Fx ;
+    inj : F ~~> Fx (* section *);
+    injK_Some {A} : forall e : F A, may_prov.(proj) (inj _ e) = Some e }.
+Arguments inj {_ _ _ _} _.
+
+Notation "F -< Fx" := (Provide Fx F)
+  (at level 92, left associativity) : type_scope.
 
 (** We provide a default instance for [MayProvide] in the form of a function
-    [proj_p] which always return [None].  We give to this default instance a
+    [proj] which always return [None].  We give to this default instance a
     ridiculously high priority number to ensure it is selected only if no other
     instances are found. *)
 
-Instance default_MayProvide (F E : effect) : MayProvide F E|1000 :=
-  { proj_p := fun _ _ => None
-  }.
+Instance default_MayProvide (F E : effect) : (E -<? F) |1000 :=
+  { proj := fun _ _ => None }.
 
 (** It is expected that, for an effect composite [Fx] which provides [F] and
-    may provide [E], [inj_p] and [proj_p] do not mix up [F] and [E]
+    may provide [E], [inj] and [proj] do not mix up [F] and [E]
     primitives. That is, injecting a primitive [e] of [F] inside [Fx], then
     projecting the resulting primitive into [E] returns [None] as long as [F]
     and [E] are two different effects. *)
 
-Class Distinguish (Fx F E : effect) `{Provide Fx F, MayProvide Fx E} : Prop :=
-  { distinguish : forall {α} (e : F α), proj_p (F := E) (inj_p (Fx := Fx) e) = None
+Class Distinguish (Fx F E : effect) `{Hp: F -< Fx, Hmp : E -<? Fx} : Prop :=
+  {
+    injK_None : forall {A} (e: F A), Hmp.(proj) (Hp.(inj) e) = None
   }.
+(* @proj Fx E H1 A (@inj Fx F H H0 A e) *)
+(* F -< Fx
+Subev -< Ev *)
 
 (** * Composing Effects *)
 
 (** We provide the [eplus] operator to compose effects together. That is,
     [eplus] can be used to build _concrete_ (as opposed to polymorphic)
     effect composite. *)
+
 
 Inductive eplus (F E : effect) (α : Type) :=
 | in_left (e : F α) : eplus F E α
@@ -122,8 +123,8 @@ Infix "+" := eplus : effect_scope.
     provide the necessary instances for the [MayProvide], [Provide] and
     [Distinguish] type classes. Note that these instances always prefer the
     left operand of [eplus]. For instance, considering a situation where
-    there is an instance for [Provide Fx F] and an instance for [Provide Ex F],
-    the instance of [Provide (Fx + Ex) F] will rely on [Fx].
+    there is an instance for [F -< Fx] and an instance for [F -< Ex],
+    the instance of [F -< (Fx + Ex)] will rely on [Fx].
 
     The main use case for [eplus] is to locally provide an additional
     effect. For instance, we can consider a [with_state] function which would
@@ -139,62 +140,55 @@ with_state true (with_state false get)
 
     will return false (that is, the variable in the inner store). *)
 
-Instance refl_MayProvide (F : effect) : MayProvide F F :=
-  { proj_p := fun _ e => Some e
+Instance refl_MayProvide (F : effect) : F -<? F :=
+  { proj := fun _ e => Some e
   }.
 
-#[program]
-Instance refl_Provide (F : effect) : @Provide F F (refl_MayProvide F) :=
-  { inj_p := fun (a : Type) (e : F a) => e
+Program Instance refl_Provide (F : effect) : F -< F :=
+  { inj := fun (a : Type) (e : F a) => e
   }.
 
-Instance eplus_left_MayProvide (Fx F E : effect) `{MayProvide Fx F}
-  : MayProvide (Fx + E) F :=
-  { proj_p := fun _ e =>
+Instance eplus_left_MayProvide (Fx F E : effect) `{F -<? Fx}
+  : F -<? (Fx + E) :=
+  { proj := fun A e => if e is in_left e then proj e else None
+                (* match e with *)
+                (* | in_left e => proj e *)
+                (* | _ => None *)
+                (* end *)
+  }.
+
+Program Instance eplus_left_Provide (Fx F E : effect) `{F -< Fx}
+  : F -< (Fx + E) :=
+  { inj := fun (a : Type) (e : F a) => in_left (inj e)
+  }.
+
+Next Obligation. by rewrite injK_Some. Qed.
+
+Instance eplus_right_MayProvide (F Ex E : effect) `{E -<? Ex}
+  : E -<? (F + Ex) :=
+  { proj := fun _ e =>
                 match e with
-                | in_left e => proj_p e
+                | in_right e => proj e
                 | _ => None
                 end
   }.
 
-#[program]
-Instance eplus_left_Provide (Fx F E : effect) `{Provide Fx F}
-  : @Provide (Fx + E) F (eplus_left_MayProvide Fx F E) :=
-  { inj_p := fun (a : Type) (e : F a) => in_left (inj_p e)
+Program Instance eplus_right_Provide (F Ex E : effect) `{E -< Ex}
+  : E -< (F + Ex) :=
+  { inj := fun _ e => in_right (inj e)
   }.
 
-Next Obligation.
-  now rewrite proj_inj_p_equ.
-Qed.
-
-Instance eplus_right_MayProvide (F Ex E : effect) `{MayProvide Ex E}
-  : MayProvide (F + Ex) E :=
-  { proj_p := fun _ e =>
-                match e with
-                | in_right e => proj_p e
-                | _ => None
-                end
-  }.
-
-#[program]
-Instance eplus_right_Provide (F Ex E : effect) `{Provide Ex E}
-  : @Provide (F + Ex) E (eplus_right_MayProvide F Ex E) :=
-  { inj_p := fun _ e => in_right (inj_p e)
-  }.
-
-Next Obligation.
-  now rewrite proj_inj_p_equ.
-Qed.
+Next Obligation. by rewrite injK_Some. Qed.
 
 (** By default, Coq's inference algorithm for type classe instances inference is
     a depth-first search. This is not without consequence in our case. For
-    instance, if we consider the search of an instance for [MayProvide (F + E)
-    E], Coq will first try [eplus_right_MayProvide] (as explained previously),
-    meaning he now search for [MayProvide F E]. It turns out such an instance
+    instance, if we consider the search of an instance for [E -<? (F + E)],
+    Coq will first try [eplus_right_MayProvide] (as explained previously),
+    meaning he now searches for [E -<? F]. It turns out such an instance
     exists: [default_MayProvide].
 
     To circumvent this issue, we write a dedicated tactic [find_may_provide]
-    which attempts to find an instance for [MayProvide (?Fx + ?Ex) ?F] with
+    which attempts to find an instance for [?F -<? (?Fx + ?Ex)] with
     [refl_MayProvide], [eplus_left_MayProvide] and [eplus_right_MayProvide]. *)
 
 Ltac find_may_provide :=
@@ -202,67 +196,54 @@ Ltac find_may_provide :=
   (eapply eplus_left_MayProvide; find_may_provide) +
   (eapply eplus_right_MayProvide; find_may_provide).
 
-#[global] Hint Extern 1 (MayProvide (eplus _ _) _) =>
+#[global] Hint Extern 1 (_ -<? (eplus _ _)) =>
   find_may_provide : typeclass_instances.
 
-#[program]
-Instance refl_Distinguish (F E : effect)
-  : @Distinguish F F E  ( @refl_MayProvide F) ( @refl_Provide F) ( @default_MayProvide F E).
+Program Instance refl_Distinguish (F E : effect)
+  : @Distinguish F F E (refl_Provide F) (default_MayProvide F E).
 
-#[program]
-Instance eplus_left_default_Distinguish (Fx Ex F E : effect)
-   `{M1 : MayProvide Fx F} `{P1 : @Provide Fx F M1}
+Program Instance eplus_left_default_Distinguish (Fx Ex F E : effect)
+   `{P1 : F -< Fx}
   : @Distinguish (Fx + Ex) F E
-                 ( @eplus_left_MayProvide Fx F Ex M1)
-                 ( @eplus_left_Provide Fx F Ex M1 P1)
-                 ( @default_MayProvide _ E).
+                 (eplus_left_Provide Fx F Ex)
+                 (default_MayProvide _ E).
 
-#[program]
-Instance eplus_right_default_Distinguish (Fx Ex F E : effect)
-   `{M1 : MayProvide Ex F} `{P1 : @Provide Ex F M1}
+Program Instance eplus_right_default_Distinguish (Fx Ex F E : effect)
+   `{P1 : F -< Ex}
   : @Distinguish (Fx + Ex) F E
-                 ( @eplus_right_MayProvide Fx Ex F M1)
-                 ( @eplus_right_Provide Fx Ex F M1 P1)
-                 ( @default_MayProvide _ E).
+                 (eplus_right_Provide Fx Ex F)
+                 (default_MayProvide _ E).
 
-#[program]
-Instance eplus_left_may_right_Distinguish (Fx Ex F E : effect)
-   `{M1 : MayProvide Fx F} `{P1 : @Provide Fx F M1} `{M2 : MayProvide Ex E}
+Program Instance eplus_left_may_right_Distinguish (Fx Ex F E : effect)
+   `{P1 : F -< Fx} `{M2 : E -<? Ex}
   : @Distinguish (Fx + Ex) F E
-                 ( @eplus_left_MayProvide Fx F Ex M1)
-                 ( @eplus_left_Provide Fx F Ex M1 P1)
-                 ( @eplus_right_MayProvide Fx Ex E M2).
+                 (eplus_left_Provide Fx F Ex)
+                 (eplus_right_MayProvide Fx Ex E).
 
-#[program]
-Instance eplus_right_may_left_Distinguish (Fx Ex F E : effect)
-   `{M1 : MayProvide Ex F} `{P1 : @Provide Ex F M1} `{M2 : MayProvide Fx E}
+Program Instance eplus_right_may_left_Distinguish (Fx Ex F E : effect)
+   `{P1 : F -< Ex} `{M2 : E -<? Fx}
   : @Distinguish (Fx + Ex) F E
-                 ( @eplus_right_MayProvide Fx Ex F M1)
-                 ( @eplus_right_Provide Fx Ex F M1 P1)
-                 ( @eplus_left_MayProvide Fx E Ex M2).
+                 (eplus_right_Provide Fx Ex F)
+                 (eplus_left_MayProvide Fx E Ex).
 
-#[program]
-Instance eplus_left_distinguish_left_Distinguish (Fx Ex F E : effect)
-   `{M1 : MayProvide Fx F} `{P1 : @Provide Fx F M1} `{M2 : MayProvide Fx E}
-   `{@Distinguish Fx F E M1 P1 M2}
+Program Instance eplus_left_distinguish_left_Distinguish (Fx Ex F E : effect)
+   `{P1 : F -< Fx} `{M2 : E -<? Fx}
+   `{@Distinguish Fx F E P1 M2}
   : @Distinguish (Fx + Ex) F E
-                 ( @eplus_left_MayProvide Fx F Ex M1)
-                 ( @eplus_left_Provide Fx F Ex M1 P1)
-                 ( @eplus_left_MayProvide Fx E Ex M2).
+                 (eplus_left_Provide Fx F Ex)
+                 (eplus_left_MayProvide Fx E Ex).
 
 Next Obligation.
-  apply distinguish.
+  apply: injK_None.
 Defined.
 
-#[program]
-Instance eplus_right_distinguish_right_Distinguish (Fx Ex F E : effect)
-   `{M1 : MayProvide Ex F} `{P1 : @Provide Ex F M1} `{M2 : MayProvide Ex E}
-   `{@Distinguish Ex F E M1 P1 M2}
+Program Instance eplus_right_distinguish_right_Distinguish (Fx Ex F E : effect)
+   `{P1 : F -< Ex} `{M2 : E -<? Ex}
+   `{@Distinguish Ex F E P1 M2}
   : @Distinguish (Fx + Ex) F E
-                 ( @eplus_right_MayProvide Fx Ex F M1)
-                 ( @eplus_right_Provide Fx Ex F M1 P1)
-                 ( @eplus_right_MayProvide Fx Ex E M2).
+                 (eplus_right_Provide Fx Ex F)
+                 (eplus_right_MayProvide Fx Ex E).
 
 Next Obligation.
-  apply distinguish.
+  apply: injK_None.
 Defined.
